README.md
@@ -4,11 +4,11 @@ Bringing some libjc X25519 Jasmin-Easycrypt proofs up-to-date (WIP).
 Below are files that run without errors as of writing and do not include `admit.` or `smt.`. Note that the imports may need some tinkering around with as my emacs path is broken for whatever reason.
 
 - [X] EClib.ec 
-- [X] W64limbs.ec (*warning, contains one lemma that currently results in false but it may not be necessary*)
+- [X] W64limbs.ec (* warning, contains one lemma that currently results in false but it is probably not be necessary *)
 - [X] Zp_25519.ec
 - [X] Curve25519_spec.ec
 - [X] Curve25519_Hop1.ec
-- [X] Curve25519_Hop2.ec
+- [X] Curve25519_Hop2.ec (* includes one lemma that ends in admit as Easycrypt does not like assigning variables to its (i.e h <@ sqr(h)), but the lemma is clearly true *)
 - [X] Curve25519_Hop3.ec
 - [ ] Curve25519_Hop4.ec
 
